src/Reflection/Z/Syntax.v
@@ -1,40 +1,50 @@
 (** * PHOAS Syntax for expression trees on ℤ *)
 Require Import Coq.ZArith.ZArith.
+Require Import Bedrock.Word.
+Require Import Crypto.Reflection.SmartMap.
 Require Import Crypto.Reflection.Syntax.
+Require Import Crypto.Reflection.TypeUtil.
 Require Import Crypto.ModularArithmetic.ModularBaseSystemListZOperations.
 Require Import Crypto.Util.FixedWordSizes.
+Require Import Crypto.Util.Option.
+Require Import Crypto.Util.NatUtil. (* for nat_beq for equality schemes *)
 Export Syntax.Notations.
 
 Local Set Boolean Equality Schemes.
 Local Set Decidable Equality Schemes.
 Inductive base_type := TZ | TWord (logsz : nat).
 
-Definition interp_base_type (v : base_type) : Type :=
-  match v with
-  | _ => Z
-  end.
+Local Notation tZ := (Tbase TZ).
+Local Notation tWord logsz := (Tbase (TWord logsz)).
 
 Inductive op : flat_type base_type -> flat_type base_type -> Type :=
-| OpConst {T} (z : interp_base_type T) : op Unit (Tbase T)
-| Add T : op (Tbase T * Tbase T) (Tbase T)
-| Sub T : op (Tbase T * Tbase T) (Tbase T)
-| Mul T : op (Tbase T * Tbase T) (Tbase T)
-| Shl T : op (Tbase T * Tbase T) (Tbase T)
-| Shr T : op (Tbase T * Tbase T) (Tbase T)
-| Land T : op (Tbase T * Tbase T) (Tbase T)
-| Lor T : op (Tbase T * Tbase T) (Tbase T)
-| Neg T (int_width : Z) : op (Tbase T) (Tbase T)
-| Cmovne T : op (Tbase T * Tbase T * Tbase T * Tbase T) (Tbase T)
-| Cmovle T : op (Tbase T * Tbase T * Tbase T * Tbase T) (Tbase T)
-| Cast T1 T2 : op (Tbase T1) (Tbase T2).
+| OpConst {T} (z : Z) : op Unit (Tbase T)
+| Add T1 T2 Tout : op (Tbase T1 * Tbase T2) (Tbase Tout)
+| Sub T1 T2 Tout : op (Tbase T1 * Tbase T2) (Tbase Tout)
+| Mul T1 T2 Tout : op (Tbase T1 * Tbase T2) (Tbase Tout)
+| Shl T1 T2 Tout : op (Tbase T1 * Tbase T2) (Tbase Tout)
+| Shr T1 T2 Tout : op (Tbase T1 * Tbase T2) (Tbase Tout)
+| Land T1 T2 Tout : op (Tbase T1 * Tbase T2) (Tbase Tout)
+| Lor T1 T2 Tout : op (Tbase T1 * Tbase T2) (Tbase Tout)
+| Neg T Tout (int_width : Z) : op (Tbase T) (Tbase Tout)
+| Cmovne T1 T2 T3 T4 Tout : op (Tbase T1 * Tbase T2 * Tbase T3 * Tbase T4) (Tbase Tout)
+| Cmovle T1 T2 T3 T4 Tout : op (Tbase T1 * Tbase T2 * Tbase T3 * Tbase T4) (Tbase Tout).
+
+Definition interp_base_type (v : base_type) : Type :=
+  match v with
+  | TZ => Z
+  | TWord logsz => wordT logsz
+  end.
 
 Definition interpToZ {t} : interp_base_type t -> Z
   := match t with
-     | _ => fun x => x
+     | TZ => fun x => x
+     | TWord _ => wordToZ
      end.
 Definition ZToInterp {t} : Z -> interp_base_type t
   := match t return Z -> interp_base_type t with
-     | _ => fun x => x
+     | TZ => fun x => x
+     | TWord _ => ZToWord
      end.
 Definition cast_const {t1 t2} (v : interp_base_type t1) : interp_base_type t2
   := ZToInterp (interpToZ v).
@@ -43,18 +53,36 @@ Local Notation eta x := (fst x, snd x).
 Local Notation eta3 x := (eta (fst x), snd x).
 Local Notation eta4 x := (eta3 (fst x), snd x).
 
-Definition interp_op src dst (f : op src dst) : interp_flat_type interp_base_type src -> interp_flat_type interp_base_type dst
-  := match f in op src dst return interp_flat_type interp_base_type src -> interp_flat_type interp_base_type dst with
-     | OpConst _ v => fun _ => v
-     | Add _ => fun xy => fst xy + snd xy
-     | Sub _ => fun xy => fst xy - snd xy
-     | Mul _ => fun xy => fst xy * snd xy
-     | Shl _ => fun xy => Z.shiftl (fst xy) (snd xy)
-     | Shr _ => fun xy => Z.shiftr (fst xy) (snd xy)
-     | Land _ => fun xy => Z.land (fst xy) (snd xy)
-     | Lor _ => fun xy => Z.lor (fst xy) (snd xy)
-     | Neg _ int_width => fun x => ModularBaseSystemListZOperations.neg int_width x
-     | Cmovne _ => fun xyzw => let '(x, y, z, w) := eta4 xyzw in cmovne x y z w
-     | Cmovle _ => fun xyzw => let '(x, y, z, w) := eta4 xyzw in cmovl x y z w
-     | Cast _ _ => cast_const
+Definition lift_op {src dst}
+           (srcv:=SmartValf (fun _ => base_type) (fun t => t) src)
+           (dstv:=SmartValf (fun _ => base_type) (fun t => t) dst)
+           (ff:=fun t0 (v : interp_flat_type _ t0) t => SmartFlatTypeMap (var':=fun _ => base_type) (fun _ _ => t) v)
+           (srcf:=ff src srcv) (dstf:=ff dst dstv)
+           (srcZ:=srcf TZ) (dstZ:=dstf TZ)
+           (opZ : interp_flat_type interp_base_type srcZ -> interp_flat_type interp_base_type dstZ)
+  : interp_flat_type interp_base_type src
+    -> interp_flat_type interp_base_type dst
+  := fun xy
+     => SmartFlatTypeMapUnInterp
+         (fun _ _ => cast_const)
+         (opZ (SmartFlatTypeMapInterp2 (fun _ _ => cast_const) _ xy)).
+
+Definition Zinterp_op src dst (f : op src dst)
+           (asZ := fun t0 => SmartFlatTypeMap (var':=fun _ => base_type) (fun _ _ => TZ) (SmartValf (fun _ => base_type) (fun t => t) t0))
+  : interp_flat_type interp_base_type (asZ src) -> interp_flat_type interp_base_type (asZ dst)
+  := match f in op src dst return interp_flat_type interp_base_type (asZ src) -> interp_flat_type interp_base_type (asZ dst) with
+     | OpConst _ v => fun _ => cast_const (t1:=TZ) v
+     | Add _ _ _ => fun xy => fst xy + snd xy
+     | Sub _ _ _ => fun xy => fst xy - snd xy
+     | Mul _ _ _ => fun xy => fst xy * snd xy
+     | Shl _ _ _ => fun xy => Z.shiftl (fst xy) (snd xy)
+     | Shr _ _ _ => fun xy => Z.shiftr (fst xy) (snd xy)
+     | Land _ _ _ => fun xy => Z.land (fst xy) (snd xy)
+     | Lor _ _ _ => fun xy => Z.lor (fst xy) (snd xy)
+     | Neg _ _ int_width => fun x => ModularBaseSystemListZOperations.neg int_width x
+     | Cmovne _ _ _ _ _ => fun xyzw => let '(x, y, z, w) := eta4 xyzw in cmovne x y z w
+     | Cmovle _ _ _ _ _ => fun xyzw => let '(x, y, z, w) := eta4 xyzw in cmovl x y z w
      end%Z.
+
+Definition interp_op src dst (f : op src dst) : interp_flat_type interp_base_type src -> interp_flat_type interp_base_type dst
+  := lift_op (Zinterp_op src dst f).
