src/Reflection/Z/Syntax/Util.v
@@ -6,23 +6,29 @@ Require Import Crypto.Reflection.TypeInversion.
 Require Import Crypto.Reflection.Z.Syntax.
 Require Import Crypto.Util.FixedWordSizesEquality.
 Require Import Crypto.Util.NatUtil.
+Require Import Crypto.Util.HProp.
 Require Import Crypto.Util.Tactics.BreakMatch.
 Require Import Crypto.Util.Tactics.DestructHead.
 Require Import Crypto.Util.Notations.
 
 Definition make_const t : interp_base_type t -> op Unit (Tbase t)
-  := OpConst.
+  := fun v => OpConst (cast_const (t2:=TZ) v).
 Definition is_const s d (v : op s d) : bool
   := match v with OpConst _ _ => true | _ => false end.
 Arguments is_const [s d] v.
-Definition is_cast s d (v : op s d) : bool
-  := match v with Cast _ _ => true | _ => false end.
-Arguments is_cast [s d] v.
 
 Definition cast_back_flat_const {var t f V}
            (v : interp_flat_type interp_base_type (@SmartFlatTypeMap base_type var f t V))
   : interp_flat_type interp_base_type t
   := @SmartFlatTypeMapUnInterp
+       _ var interp_base_type interp_base_type
+       f (fun _ _ => cast_const)
+       t V v.
+
+Definition cast_flat_const {var t f V}
+           (v : interp_flat_type interp_base_type t)
+  : interp_flat_type interp_base_type (@SmartFlatTypeMap base_type var f t V)
+  := @SmartFlatTypeMapInterp2
        _ var interp_base_type interp_base_type
        f (fun _ _ => cast_const)
        t V v.
@@ -41,33 +47,27 @@ Global Arguments base_type_max !_ !_ / .
 Global Arguments TypeUtil.base_type_min _ _ _ /  _.
 Global Arguments TypeUtil.base_type_max _ _ _ /  _.
 
-Definition Castb {var} A A' (v : exprf base_type op (var:=var) (Tbase A))
-  : exprf base_type op (var:=var) (Tbase A')
-  := Op (Cast A A') v.
-
-Local Notation Se opv := (Some (existT _ (_, _) opv)) (only parsing).
-
-Definition genericize_op src dst (opc : op src dst) (t_in t_out : base_type)
-  : option { src'dst' : _ & op (fst src'dst') (snd src'dst') }
+Definition genericize_op {var' src dst} (opc : op src dst) {f}
+  : forall {vs vd}, op (@SmartFlatTypeMap _ var' f src vs) (@SmartFlatTypeMap _ var' f dst vd)
   := match opc with
-     | OpConst T z => Se (OpConst z)
-     | Add T => Se (Add t_out)
-     | Sub T => Se (Sub t_in)
-     | Mul T => Se (Mul t_out)
-     | Shl T => Se (Shl t_out)
-     | Shr T => Se (Shr t_in)
-     | Land T => Se (Land t_out)
-     | Lor T => Se (Lor t_out)
-     | Neg T int_width => Se (Neg t_out int_width)
-     | Cmovne T => Se (Cmovne t_out)
-     | Cmovle T => Se (Cmovle t_out)
-     | Cast T1 T2 => None
+     | OpConst _ z => fun _ _ => OpConst z
+     | Add _ _ _ => fun _ _ => Add _ _ _
+     | Sub _ _ _ => fun _ _ => Sub _ _ _
+     | Mul _ _ _ => fun _ _ => Mul _ _ _
+     | Shl _ _ _ => fun _ _ => Shl _ _ _
+     | Shr _ _ _ => fun _ _ => Shr _ _ _
+     | Land _ _ _ => fun _ _ => Land _ _ _
+     | Lor _ _ _ => fun _ _ => Lor _ _ _
+     | Neg _ _ int_width => fun _ _ => Neg _ _ int_width
+     | Cmovne _ _ _ _ _ => fun _ _ => Cmovne _ _ _ _ _
+     | Cmovle _ _ _ _ _ => fun _ _ => Cmovle _ _ _ _ _
      end.
 
 Lemma cast_const_id {t} v
   : @cast_const t t v = v.
 Proof.
   destruct t; simpl; trivial.
+  rewrite ZToWord_wordToZ; reflexivity.
 Qed.
 
 Lemma cast_const_idempotent {a b c} v
@@ -96,20 +96,77 @@ Proof.
     intro; rewrite ?ZToWord_wordToZ; reflexivity.
 Qed.
 
-Lemma is_cast_correct s d opc
-  : forall e,
-    @is_cast (Tbase s) (Tbase d) opc = true
-    -> Syntax.interp_op _ _ opc (interpf Syntax.interp_op e)
-       = interpf Syntax.interp_op (Castb s d e).
+Local Notation iffT A B := ((A -> B) * (B -> A))%type (only parsing).
+
+Section unzify.
+  Context {var'} {f : forall t : base_type, var' t -> base_type}.
+  Let asZ := fun t => SmartFlatTypeMap
+                        (fun _ _ => TZ)
+                        (SmartValf (fun _ => base_type) (fun t => t) t).
+  Definition unzify_op_helper_step
+             (unzify_op_helper
+              : forall {t : flat_type base_type}
+                       {vs : interp_flat_type var' t},
+                 iffT (interp_flat_type
+                         interp_base_type
+                         (asZ t))
+                      (interp_flat_type
+                         interp_base_type
+                         (asZ (SmartFlatTypeMap f vs))))
+             {t : flat_type base_type}
+    : forall {vs : interp_flat_type var' t},
+      iffT (interp_flat_type
+              interp_base_type
+              (asZ t))
+           (interp_flat_type
+              interp_base_type
+              (asZ (SmartFlatTypeMap f vs)))
+    := match t with
+       | Tbase T => fun _ => (fun x => x, fun x => x)
+       | Unit => fun _ => (fun x => x, fun x => x)
+       | Prod A B
+         => fun (vs : interp_flat_type _ A * interp_flat_type _ B)
+            => let f1 := @unzify_op_helper A (fst vs) in
+               let f2 := @unzify_op_helper B (snd vs) in
+               ((fun x : interp_flat_type _ (asZ A) * interp_flat_type _ (asZ B)
+                 => (fst f1 (fst x), fst f2 (snd x))),
+                (fun x : interp_flat_type _ (asZ (SmartFlatTypeMap f (fst vs)))
+                         * interp_flat_type _ (asZ (SmartFlatTypeMap f (snd vs)))
+                 => (snd f1 (fst x), snd f2 (snd x))))
+       end.
+  Fixpoint unzify_op_helper {t vs}
+    := @unzify_op_helper_step (@unzify_op_helper) t vs.
+
+  Definition unzify_op
+             {src dst : flat_type base_type}
+             {vs : interp_flat_type var' src} {vd : interp_flat_type var' dst}
+             (F : interp_flat_type interp_base_type (asZ src) -> interp_flat_type interp_base_type (asZ dst))
+             (x : interp_flat_type interp_base_type (asZ (SmartFlatTypeMap f vs)))
+    : interp_flat_type interp_base_type (asZ (SmartFlatTypeMap f vd))
+    := fst unzify_op_helper (F (snd unzify_op_helper x)).
+End unzify.
+
+Arguments unzify_op_helper_step _ _ _ !_ _ / .
+Arguments unzify_op_helper _ _ !_ _ / .
+
+Lemma Zinterp_op_genericize_op {var' src dst opc f vs vd}
+  : Zinterp_op _ _ (@genericize_op var' src dst opc f vs vd)
+    = unzify_op (Zinterp_op _ _ opc).
 Proof.
-  preinvert_one_type opc; intros ? opc.
-  pose (fun x y => op y x) as op'.
-  change op with (fun x y => op' y x) in opc; cbv beta in opc.
-  preinvert_one_type opc; intros ? opc; subst op'; cbv beta in *.
-  destruct opc; try exact I; simpl; try congruence.
+  destruct opc; unfold unzify_op; reflexivity.
 Qed.
 
-Lemma wff_Castb {var1 var2 G A A'} {e1 e2 : exprf base_type op (Tbase A)}
-      (Hwf : wff (var1:=var1) (var2:=var2) G e1 e2)
-  : wff G (Castb A A' e1) (Castb A A' e2).
-Proof. constructor; assumption. Qed.
+Lemma lift_op_prod_dst {src dstA dstB}
+      {f : _ -> interp_flat_type _ (SmartFlatTypeMap _ (SmartValf _ _ _)) * interp_flat_type _ (SmartFlatTypeMap _ (SmartValf _ _ _))}
+      {x}
+  : @lift_op src (Prod dstA dstB) f x
+    = (@lift_op src dstA (fun y => fst (f y)) x, @lift_op src dstB (fun y => snd (f y)) x).
+Proof. reflexivity. Qed.
+
+Lemma cast_back_flat_const_prod {var A B f} {V : _ * _}
+      (v : interp_flat_type interp_base_type (@SmartFlatTypeMap base_type var f A (fst V))
+           * interp_flat_type interp_base_type (@SmartFlatTypeMap base_type var f B (snd V)))
+  : @cast_back_flat_const var (Prod A B) f V v
+    = (@cast_back_flat_const var A f (fst V) (fst v),
+       @cast_back_flat_const var B f (snd V) (snd v)).
+Proof. reflexivity. Qed.
