src/Reflection/Z/Bounds/MapCastByDeBruijn.v
@@ -5,10 +5,6 @@ Require Import Crypto.Reflection.Z.Syntax.Util.
 Require Import Crypto.Reflection.Z.Bounds.Interpretation.
 
 Section language.
-  Context (genericize_op : forall t tR (opc : op t tR)
-                                  (args_bs : interp_flat_type Bounds.interp_base_type t),
-              op (SmartMap.SmartFlatTypeMap (fun _ => Bounds.bounds_to_base_type) args_bs)
-                 (SmartMap.SmartFlatTypeMap (fun _ => Bounds.bounds_to_base_type) (Bounds.interp_op opc args_bs))).
   Context {t : type base_type}.
 
   Definition MapCastCompile := @MapCastCompile t.
@@ -16,7 +12,7 @@ Section language.
     := @MapCastDoCast
          (@Bounds.interp_base_type) (@Bounds.interp_op)
          (fun _ => @Bounds.bounds_to_base_type)
-         (fun _ _ opc _ => @genericize_op _ _ opc _)
+         (fun _ _ opc _ => @genericize_op _ _ _ opc _ _ _)
          t.
   Definition MapCastDoInterp
     := @MapCastDoInterp
