src/Reflection/Z/Bounds/MapCastByDeBruijnInterp.v
@@ -1,0 +1,25 @@
+Require Import Crypto.Reflection.Syntax.
+Require Import Crypto.Reflection.Wf.
+Require Import Crypto.Reflection.SmartMap.
+Require Import Crypto.Reflection.Relations.
+Require Import Crypto.Reflection.Z.MapCastByDeBruijnInterp.
+Require Import Crypto.Reflection.Z.Syntax.
+Require Import Crypto.Reflection.Z.Syntax.Util.
+Require Import Crypto.Reflection.Z.Bounds.Interpretation.
+Require Import Crypto.Reflection.Z.Bounds.InterpretationLemmas.
+Require Import Crypto.Reflection.Z.Bounds.MapCastByDeBruijn.
+
+Lemma MapCastCorrect
+      {t} (e : Expr base_type op t)
+      (Hwf : Wf e)
+      (input_bounds : interp_flat_type Bounds.interp_base_type (domain t))
+  : forall {b} e' (He':MapCast e input_bounds = Some (existT _ b e'))
+           v v' (Hv : Bounds.is_bounded_by input_bounds v /\ cast_back_flat_const v' = v),
+    Interp (@Bounds.interp_op) e input_bounds = b
+    /\ Bounds.is_bounded_by b (Interp interp_op e v)
+    /\ cast_back_flat_const (Interp interp_op e' v') = (Interp interp_op e v).
+Proof.
+  apply MapCastCorrect; auto.
+  { apply is_bounded_by_interp_op. }
+  { apply pull_cast_genericize_op. }
+Qed.
