src/Reflection/Z/Bounds/Pipeline/ReflectiveTactics.v
@@ -1,0 +1,168 @@
+(** * Reflective Pipeline: Tactics that execute the pipeline *)
+Require Import Crypto.Reflection.Syntax.
+Require Import Crypto.Reflection.Wf.
+Require Import Crypto.Reflection.WfReflective.
+Require Import Crypto.Reflection.RenameBinders.
+Require Import Crypto.Reflection.Z.Syntax.
+Require Import Crypto.Reflection.Z.Syntax.Util.
+Require Import Crypto.Reflection.Z.Bounds.Interpretation.
+Require Import Crypto.Reflection.Z.Bounds.Relax.
+Require Import Crypto.Reflection.Reify.
+Require Import Crypto.Reflection.Z.Reify.
+Require Import Crypto.Reflection.Z.Bounds.Pipeline.PreDefinitions.
+Require Import Crypto.Reflection.Z.Bounds.Pipeline.Definition.
+Require Import Crypto.Util.Tactics.Head.
+Require Import Crypto.Util.Tactics.SubstLet.
+Require Import Crypto.Util.Option.
+
+Module Export Exports.
+  Export Crypto.Reflection.Reify. (* export for the instances for recursing under binders *)
+  Export Crypto.Reflection.Z.Reify. (* export for the tactic redefinitions *)
+End Exports.
+
+Ltac rexpr_cbv :=
+  lazymatch goal with
+  | [ |- { rexpr | forall x, Interp _ (t:=?T) rexpr x = ?uncurry ?oper x } ]
+    => let operf := head oper in
+       let uncurryf := head uncurry in
+       try cbv delta [T]; try cbv delta [oper];
+       try cbv beta iota delta [uncurryf]
+  | [ |- { rexpr | forall x, Interp _ (t:=?T) rexpr x = ?oper x } ]
+    => let operf := head oper in
+       try cbv delta [T]; try cbv delta [oper]
+  end;
+  cbv beta iota delta [interp_flat_type interp_base_type].
+Ltac reify_sig :=
+  rexpr_cbv; eexists; Reify_rhs; reflexivity.
+Ltac assert_reflective :=
+  lazymatch goal with
+  | [ |- @Bounds.is_bounded_by (codomain ?T) ?bounds _
+         /\ cast_back_flat_const ?fW = ?fZ (cast_back_flat_const ?v) ]
+    => let rexpr := fresh "rexpr" in
+       simple refine (let rexpr : { rexpr | forall x, Interp interp_op (t:=T) rexpr x = fZ x } := _ in _);
+       [ cbv [interp_flat_type interp_base_type Tuple.tuple Tuple.tuple'] in *;
+         subst fW
+       | rewrite <- (proj2_sig rexpr);
+         let rexpr' := fresh rexpr in
+         set (rexpr' := proj1_sig rexpr);
+         unfold proj1_sig in rexpr';
+         subst rexpr fZ ]
+  end.
+Ltac prove_rexpr_wfT
+  := reflect_Wf Equality.base_type_eq_semidec_is_dec Equality.op_beq_bl.
+
+Ltac assert_wf :=
+  lazymatch goal with
+  | [ |- @Bounds.is_bounded_by (codomain ?T) ?bounds _
+         /\ cast_back_flat_const ?fW = Interp _ ?fZ (@cast_back_flat_const _ _ _ ?input_bounds ?v) ]
+    => assert (Wf fZ) by (clear; prove_rexpr_wfT)
+  end.
+
+Notation rexpr_post_wf_pipeline_option rexprZ rexpr_bounds
+  := (PostWfPipeline rexprZ rexpr_bounds)
+       (only parsing).
+Notation rexpr_post_wf_pipeline_postprocess1 v
+  := (invert_Some v)
+       (only parsing).
+Notation get_output_type v := (OutputType v) (only parsing).
+Notation get_bounds v := (@output_bounds v) (only parsing).
+Notation get_output_expr v := (@output_expr v) (only parsing).
+Notation rexpr_post_wf_pipeline_postprocess2 v
+  := (renamify v)
+       (only parsing).
+
+Notation rexpr_correct_and_bounded rexprZ rexprW input_bounds output_bounds rexprZ_Wf
+  := (fun v v' Hv
+      => proj2
+           (@PostWfPipelineCorrct
+              _ rexprZ input_bounds rexprZ_Wf
+              output_bounds rexprW
+              _
+              v v' Hv))
+       (only parsing).
+
+Ltac rexpr_correct_and_bounded_obligation_tac :=
+  intros; subst_let; clear;
+  lazymatch goal with
+  | [ |- ?x = Some ?y ]
+    => abstract vm_cast_no_check (eq_refl (Some y))
+  | _ => vm_compute; constructor
+  end.
+
+
+Ltac make_correctness rexprZ bounds Hcorrectness :=
+  let rexprW_pkgo := (eval vm_compute in (rexpr_post_wf_pipeline_option rexprZ bounds)) in
+  let rexprW_pkg := (eval vm_compute in (rexpr_post_wf_pipeline_postprocess1 rexprW_pkgo)) in
+  let rexprT := constr:(get_output_type rexprW_pkg) in
+  let rexprW' := (eval vm_compute in (get_output_expr rexprW_pkg)) in
+  let rexprW := (eval cbv beta iota zeta in (rexpr_post_wf_pipeline_postprocess2 rexprW')) in
+  let rexpr_output_bounds := (eval vm_compute in (get_bounds rexprW_pkg)) in
+  let rexprZ_Wf := lazymatch goal with H : Wf rexprZ |- _ => H end in
+  simple refine (let Hcorrectness := rexpr_correct_and_bounded rexprZ rexprW bounds rexpr_output_bounds rexprZ_Wf in _);
+  [ rexpr_correct_and_bounded_obligation_tac.. | clearbody Hcorrectness ].
+Ltac do_pose_correctness Hcorrectness :=
+  lazymatch goal with
+  | [ |- @Bounds.is_bounded_by (codomain ?T) ?bounds _
+         /\ cast_back_flat_const ?fW = Interp _ ?fZ (@cast_back_flat_const _ _ _ ?input_bounds ?v) ]
+    => make_correctness fZ input_bounds Hcorrectness
+  end.
+Ltac pretighten_bounds tighter_bounds :=
+  lazymatch goal with
+  | [ |- @Bounds.is_bounded_by ?t ?relaxed_bounds _ /\ cast_back_flat_const ?v = ?k ]
+    => simple refine (@relax_output_bounds t tighter_bounds relaxed_bounds _ v k _ _)
+  end.
+Ltac posttighten_bounds :=
+  [ > clear; vm_compute; reflexivity | unfold eq_rect | clear; abstract vm_cast_no_check (eq_refl true) ].
+Ltac pretighten_bounds_from_correctness Hcorrectness :=
+  cbv beta iota zeta in Hcorrectness;
+  lazymatch type of Hcorrectness with
+  | forall v v', _ -> Bounds.is_bounded_by ?tighter_bounds _ /\ _
+    => pretighten_bounds tighter_bounds
+  end.
+Ltac tighten_bounds_from_correctness Hcorrectness :=
+  pretighten_bounds_from_correctness Hcorrectness; posttighten_bounds.
+Ltac specialize_Hcorrectness Hcorrectness :=
+  lazymatch goal with
+  | [ |- @Bounds.is_bounded_by (codomain ?T) ?bounds (Interp _ ?fZ ?v')
+         /\ cast_back_flat_const ?fW = Interp _ ?fZ ?v' ]
+    => let v := lazymatch v' with cast_back_flat_const ?v => v end in
+       specialize (Hcorrectness v' v);
+       lazymatch type of Hcorrectness with
+       | ?T -> Bounds.is_bounded_by _ _ /\ cast_back_flat_const ?fW' = _
+         => let fWev := (eval cbv delta [fW] in fW) in
+            unify fWev fW'; cut T
+       end;
+       [ let H := fresh in intro H; specialize (Hcorrectness H) | ]
+  end.
+Ltac handle_bounds_from_hyps :=
+  repeat match goal with
+         | _ => assumption
+         | [ |- cast_back_flat_const _ = cast_back_flat_const _ ] => reflexivity
+         | [ |- _ /\ _ ] => split
+         | [ |- Bounds.is_bounded_by (_, _) _ ] => split
+         end.
+Ltac do_pre_wf_pipeline :=
+  lazymatch goal with
+  | [ |- @Bounds.is_bounded_by (codomain ?T) ?bounds (Interp _ ?fZ ?v')
+         /\ cast_back_flat_const ?fW = Interp _ ?fZ ?v' ]
+    => rewrite <- !(InterpPreWfPipeline fZ);
+       let fZ' := fresh fZ in
+       rename fZ into fZ';
+       set (fZ := PreWfPipeline fZ');
+       vm_compute in fZ; clear fZ'
+  end.
+Ltac do_reify := [ > reify_sig | cbv beta iota in * ].
+Ltac do_post_wf_pipeline :=
+  let Hcorrectness := fresh "Hcorrectness" in
+  do_pose_correctness Hcorrectness;
+  tighten_bounds_from_correctness Hcorrectness;
+  specialize_Hcorrectness Hcorrectness;
+  [ exact Hcorrectness
+  | handle_bounds_from_hyps ].
+
+Ltac do_reflective_pipeline :=
+  assert_reflective;
+  do_reify;
+  do_pre_wf_pipeline;
+  assert_wf;
+  do_post_wf_pipeline.
