src/Reflection/Z/Reify.v
@@ -15,19 +15,19 @@ Require Import Crypto.Reflection.EtaInterp.
 
 Ltac base_reify_op op op_head extra ::=
      lazymatch op_head with
-     | @Z.add => constr:(reify_op op op_head 2 (Add TZ))
-     | @Z.mul => constr:(reify_op op op_head 2 (Mul TZ))
-     | @Z.sub => constr:(reify_op op op_head 2 (Sub TZ))
-     | @Z.shiftl => constr:(reify_op op op_head 2 (Shl TZ))
-     | @Z.shiftr => constr:(reify_op op op_head 2 (Shr TZ))
-     | @Z.land => constr:(reify_op op op_head 2 (Land TZ))
-     | @Z.lor => constr:(reify_op op op_head 2 (Lor TZ))
-     | @ModularBaseSystemListZOperations.cmovne => constr:(reify_op op op_head 4 (Cmovne TZ))
-     | @ModularBaseSystemListZOperations.cmovl => constr:(reify_op op op_head 4 (Cmovle TZ))
+     | @Z.add => constr:(reify_op op op_head 2 (Add TZ TZ TZ))
+     | @Z.mul => constr:(reify_op op op_head 2 (Mul TZ TZ TZ))
+     | @Z.sub => constr:(reify_op op op_head 2 (Sub TZ TZ TZ))
+     | @Z.shiftl => constr:(reify_op op op_head 2 (Shl TZ TZ TZ))
+     | @Z.shiftr => constr:(reify_op op op_head 2 (Shr TZ TZ TZ))
+     | @Z.land => constr:(reify_op op op_head 2 (Land TZ TZ TZ))
+     | @Z.lor => constr:(reify_op op op_head 2 (Lor TZ TZ TZ))
+     | @ModularBaseSystemListZOperations.cmovne => constr:(reify_op op op_head 4 (Cmovne TZ TZ TZ TZ TZ))
+     | @ModularBaseSystemListZOperations.cmovl => constr:(reify_op op op_head 4 (Cmovle TZ TZ TZ TZ TZ))
      | @ModularBaseSystemListZOperations.neg
        => lazymatch extra with
           | @ModularBaseSystemListZOperations.neg ?int_width _
-            => constr:(reify_op op op_head 1 (Neg TZ int_width))
+            => constr:(reify_op op op_head 1 (Neg TZ TZ int_width))
           | _ => fail 100 "Anomaly: In Reflection.Z.base_reify_op: head is neg but body is wrong:" extra
           end
      end.
@@ -38,19 +38,12 @@ Ltac base_reify_type T ::=
 Ltac Reify' e := Reflection.Reify.Reify' base_type interp_base_type op e.
 Ltac Reify e :=
   let v := Reflection.Reify.Reify base_type interp_base_type op make_const e in
-  constr:(ExprEta ((*Inline _*) ((*CSE _*) (InlineConst is_const (Linearize v))))).
-Ltac prove_ExprEta_InlineConst_Linearize_Compile_correct :=
+  constr:(ExprEta v).
+Ltac prove_ExprEta_Compile_correct :=
   fun _
   => intros;
      rewrite ?InterpExprEta;
-     lazymatch goal with
-     | [ |- ?R (@Syntax.Interp ?base_type_code ?interp_base_type ?op ?interp_op ?t (InlineConst ?is_const (Linearize _)) ?x) _ ]
-       => etransitivity;
-          [ apply (@InterpInlineConst base_type_code interp_base_type op interp_op is_const t);
-            reflect_Wf base_type_eq_semidec_is_dec op_beq_bl
-          | etransitivity;
-            [ apply (@InterpLinearize base_type_code interp_base_type op interp_op t)
-            | prove_compile_correct_using ltac:(fun _ => apply make_const_correct) () ] ]
-     end.
+     prove_compile_correct_using ltac:(fun _ => apply make_const_correct) ().
+
 Ltac Reify_rhs :=
-  Reflection.Reify.Reify_rhs_gen Reify prove_ExprEta_InlineConst_Linearize_Compile_correct interp_op ltac:(fun tac => tac ()).
+  Reflection.Reify.Reify_rhs_gen Reify prove_ExprEta_Compile_correct interp_op ltac:(fun tac => tac ()).
